Given_Clause_Loops/Fair_Zipperposition_Loop_without_Ghosts.thy
@@ -164,6 +164,7 @@ proof -
 
   have sts: "Sts = Sts'" if "Sts' = lmap wo_ghosts_of Sts0" for Sts'
     using that
+(*
   proof (coinduction arbitrary: Sts Sts' rule: llist.coinduct)
     case Eq_llist
 
@@ -190,6 +191,8 @@ proof -
     ultimately show ?case
       by fastforce
   qed
+*)
+    sorry
 
   have chain0: "chain (\<leadsto>ZLf) Sts0"
     sorry
@@ -273,7 +276,7 @@ locale fifo_zipperposition_loop =
     countable_Inf_between: "finite A \<Longrightarrow> countable (no_labels.Inf_between A {C})"
 begin
 
-sublocale fifo_passive_set
+sublocale fifo_prover_queue
   .
 
 sublocale fair_zipperposition_loop Bot_F Inf_F Bot_G Q entails_q Inf_G_q Red_I_q Red_F_q \<G>_F_q \<G>_I_q
